backend/Constpropproof.v
@@ -125,6 +125,7 @@ Lemma transf_ros_correct:
      find_function tge (transf_ros ae ros) rs' = Some (transf_fundef (romem_for cunit) f)
   /\ linkorder cunit prog.
 Proof.
+  unfold find_function.
   intros until rs'; intros GE EM FF RLD. destruct ros; simpl in *.
 - (* function pointer *)
   generalize (EM r); fold (areg ae r); intro VM. generalize (RLD r); intro LD.
@@ -133,7 +134,7 @@ Proof.
        find_function tge (inl _ r) rs' = Some (transf_fundef (romem_for cunit) f)
     /\ linkorder cunit prog).
   {
-    simpl. inv LD. apply functions_translated; auto. rewrite <- H0 in FF; discriminate.
+    simpl. inv LD. apply functions_translated; auto. congruence. rewrite <- H0 in FF; discriminate.
   }
   destruct (areg ae r); auto. destruct p; auto.
   predSpec Ptrofs.eq Ptrofs.eq_spec ofs Ptrofs.zero; intros; auto.
@@ -159,6 +160,7 @@ Lemma transf_ros_correct_ptr:
   regs_lessdef rs rs' ->
   find_function_ptr tge (transf_ros ae ros) rs' = Some vf.
 Proof.
+  unfold find_function.
   intros until rs'; intros GE EM FF FF' RLD. destruct ros; simpl in *.
 - (* function pointer *)
   generalize (EM r); fold (areg ae r); intro VM. generalize (RLD r); intro LD.
@@ -346,12 +348,12 @@ Qed.
 
 Inductive match_stackframes: stackframe -> stackframe -> Prop :=
    match_stackframe_intro:
-      forall res sp pc rs f rs' cu,
+      forall res sp pc rs ty cp f rs' cu,
       linkorder cu prog ->
       regs_lessdef rs rs' ->
     match_stackframes
-        (Stackframe res f sp pc rs)
-        (Stackframe res (transf_function (romem_for cu) f) sp pc rs').
+        (Stackframe res ty cp f sp pc rs)
+        (Stackframe res ty cp (transf_function (romem_for cu) f) sp pc rs').
 
 Inductive match_states: nat -> state -> state -> Prop :=
   | match_states_intro:
@@ -372,13 +374,13 @@ Inductive match_states: nat -> state -> state -> Prop :=
       match_states O (Callstate s f args m)
                      (Callstate s' (transf_fundef (romem_for cu) f) args' m')
   | match_states_return:
-      forall s v m s' v' m' ty cp
+      forall s v m s' v' m'
            (STACKS: list_forall2 match_stackframes s s')
            (RES: Val.lessdef v v')
            (MEM: Mem.extends m m'),
       list_forall2 match_stackframes s s' ->
-      match_states O (Returnstate s v m ty cp)
-                     (Returnstate s' v' m' ty cp).
+      match_states O (Returnstate s v m)
+                     (Returnstate s' v' m').
 
 Lemma match_states_succ:
   forall s f sp pc rs m s' rs' m' cu,
@@ -559,6 +561,7 @@ Proof.
   eapply call_trace_lessdef; eauto using senv_preserved, symbols_preserved.
   apply regs_lessdef_regs; auto.
   constructor; auto. constructor; auto.
+  rewrite <- find_comp_translated.
   econstructor; eauto.
   apply regs_lessdef_regs; auto.
 
@@ -652,7 +655,7 @@ Opaque builtin_strength_reduction.
 
 - (* Ireturn *)
   exploit Mem.free_parallel_extends; eauto. intros [m2' [A B]].
-  left; exists O; exists (Returnstate s' (regmap_optget or Vundef rs') m2' (sig_res (fn_sig (transf_function (romem_for cu) f))) (comp_of (transf_function (romem_for cu) f))); split.
+  left; exists O; exists (Returnstate s' (regmap_optget or Vundef rs') m2'); split.
   eapply exec_Ireturn; eauto. TransfInstr; auto.
   constructor; auto.
   destruct or; simpl; auto.
@@ -677,7 +680,7 @@ Opaque builtin_strength_reduction.
   constructor; auto.
 
 - (* return *)
-  inv H6. inv H1.
+  inv H4. inv H1.
   left; exists O; econstructor; split.
   eapply exec_return; eauto.
   rewrite comp_transf_function. intros G. specialize (NO_CROSS_PTR G).
