backend/RTL.v
@@ -195,16 +195,16 @@ Section RELSEM.
 
 Variable ge: genv.
 
-Definition find_function
-      (ros: reg + ident) (rs: regset) : option fundef :=
-  match ros with
-  | inl r => Genv.find_funct ge rs#r
-  | inr symb =>
-      match Genv.find_symbol ge symb with
-      | None => None
-      | Some b => Genv.find_funct_ptr ge b
-      end
-  end.
+(* Definition find_function *)
+(*       (ros: reg + ident) (rs: regset) : option fundef := *)
+(*   match ros with *)
+(*   | inl r => Genv.find_funct ge rs#r *)
+(*   | inr symb => *)
+(*       match Genv.find_symbol ge symb with *)
+(*       | None => None *)
+(*       | Some b => Genv.find_funct_ptr ge b *)
+(*       end *)
+(*   end. *)
 
 Definition find_function_ptr ros rs :=
   match ros with
@@ -213,6 +213,12 @@ Definition find_function_ptr ros rs :=
                | Some b => Some  (Vptr b Ptrofs.zero)
                | None => None
                end
+  end.
+
+Definition find_function (ros: reg + ident) (rs: regset): option fundef :=
+  match find_function_ptr ros rs with
+  | Some v => Genv.find_funct ge v
+  | None => None
   end.
 
 Lemma find_function_find_function_ptr:
